...

src/Init/Data/List/Basic.lean
@@ -962,6 +962,26 @@ def IsInfix (l₁ : List α) (l₂ : List α) : Prop := Exists fun s => Exists f
 
 @[inherit_doc] infixl:50 " <:+: " => IsInfix
 
+/-! ### splitAt -/
+
+/--
+Split a list at an index.
+```
+splitAt 2 [a, b, c] = ([a, b], [c])
+```
+-/
+def splitAt (n : Nat) (l : List α) : List α × List α := go l n [] where
+  /--
+  Auxiliary for `splitAt`:
+  `splitAt.go l xs n acc = (acc.reverse ++ take n xs, drop n xs)` if `n < xs.length`,
+  and `(l, [])` otherwise.
+  -/
+  go : List α → Nat → List α → List α × List α
+  | [], _, _ => (l, []) -- This branch ensures the pointer equality of the result with the input
+                        -- without any runtime branching cost.
+  | x :: xs, n+1, acc => go xs n (x :: acc)
+  | xs, _, acc => (acc.reverse, xs)
+
 /-! ### rotateLeft -/
 
 /--
