src/Init/Data/List/Sort/Basic.lean
@@ -1,0 +1,468 @@
+/-
+Copyright (c) 2024 Lean FRO. All rights reserved.
+Released under Apache 2.0 license as described in the file LICENSE.
+Authors: Kim Morrison
+-/
+prelude
+
+import Init.Data.List.Nat.Sublist
+import Init.Data.List.Nat.Pairwise
+import Init.Data.List.Nat.Range
+import Init.Data.List.Perm
+import Init.Data.List.Impl
+-- import Lean.Eval
+
+namespace List
+
+/--
+`O(min |l| |r|)`. Merge two lists using `le` as a switch.
+
+This version is not tail-recursive,
+but it is replaced at runtime by `mergeTR` using a `@[csimp]` lemma.
+-/
+def merge (le : α → α → Bool) : List α → List α → List α
+  | [], ys => ys
+  | xs, [] => xs
+  | x :: xs, y :: ys =>
+    if le x y then
+      x :: merge le xs (y :: ys)
+    else
+      y :: merge le (x :: xs) ys
+
+/--
+Split a list in two equal parts. If the length is odd, the first part will be one element longer.
+-/
+def splitInTwo (l : { l : List α // l.length = n }) :
+    { l : List α // l.length = (n+1)/2 } × { l : List α // l.length = n/2 } :=
+  let r := splitAt ((n+1)/2) l.1
+  (⟨r.1, by simp [r, splitAt_eq, l.2]; omega⟩, ⟨r.2, by simp [r, splitAt_eq, l.2]; omega⟩)
+
+/--
+Simplified implementation of stable merge sort.
+
+This function is designed for reasoning about the algorithm, and is not efficient.
+(It particular it uses the non tail-recursive `merge` function,
+and so can not be run on large lists, but also makes unnecessary traversals of lists.)
+It is replaced at runtime in the compiler by `mergeSortTR₂` using a `@[csimp]` lemma.
+
+Because we want the sort to be stable,
+it is essential that we split the list in two contiguous sublists.
+-/
+def mergeSort (le : α → α → Bool) : List α → List α
+  | [] => []
+  | [a] => [a]
+  | a :: b :: xs =>
+    let lr := splitInTwo ⟨a :: b :: xs, rfl⟩
+    have := by simpa using lr.2.2
+    have := by simpa using lr.1.2
+    merge le (mergeSort le lr.1) (mergeSort le lr.2)
+termination_by l => l.length
+
+abbrev Sorted (le : α → α → Prop) (xs : List α) : Prop := xs.Pairwise le
+
+-- instance boolPredToPred : Coe (α → Bool) (α  → Prop) where
+--   coe r := fun a => r a = true
+-- instance boolRelToRel : Coe (α → α → Bool) (α → α → Prop) where
+--   coe r := fun a b => r a b = true
+
+@[simp] theorem splitInTwo_fst (l : { l : List α // l.length = n }) : (splitInTwo l).1 = ⟨l.1.take ((n+1)/2), by simp [splitInTwo, splitAt_eq, l.2]; omega⟩ := by
+  simp [splitInTwo, splitAt_eq]
+
+@[simp] theorem splitInTwo_snd (l : { l : List α // l.length = n }) : (splitInTwo l).2 = ⟨l.1.drop ((n+1)/2), by simp [splitInTwo, splitAt_eq, l.2]; omega⟩ := by
+  simp [splitInTwo, splitAt_eq]
+
+theorem splitInTwo_fst_append_splitInTwo_snd (l : { l : List α // l.length = n }) : (splitInTwo l).1.1 ++ (splitInTwo l).2.1 = l.1 := by
+  simp
+
+variable {le : α → α → Bool}
+
+@[simp] theorem merge_nil_right (xs : List α) : merge le xs [] = xs := by
+  induction xs with
+  | nil => simp [merge]
+  | cons x xs ih => simp [merge, ih]
+
+
+
+theorem mem_merge {a : α} {xs ys : List α} : a ∈ merge le xs ys ↔ a ∈ xs ∨ a ∈ ys := by
+  induction xs generalizing ys with
+  | nil => simp [merge]
+  | cons x xs ih =>
+    induction ys with
+    | nil => simp [merge]
+    | cons y ys ih =>
+      simp only [merge]
+      split <;> rename_i h
+      · simp_all [or_assoc]
+      · simp only [mem_cons, or_assoc, Bool.not_eq_true, ih, ← or_assoc]
+        apply or_congr_left
+        simp only [or_comm (a := a = y), or_assoc]
+
+theorem merge_sorted
+    (trans : ∀ (a b c : α), le a b → le b c → le a c)
+    (total : ∀ (a b : α), !le a b → le b a)
+    (l₁ l₂ : List α) (h₁ : l₁.Sorted le) (h₂ : l₂.Sorted le) : (merge le l₁ l₂).Sorted le := by
+  induction l₁ generalizing l₂ with
+  | nil => simpa only [merge]
+  | cons x l₁ ih₁ =>
+    induction l₂ with
+    | nil => simpa only [merge]
+    | cons y l₂ ih₂ =>
+      simp only [merge]
+      split <;> rename_i h
+      · apply Pairwise.cons
+        · intro z m
+          rw [mem_merge, mem_cons] at m
+          rcases m with (m|rfl|m)
+          · exact rel_of_pairwise_cons h₁ m
+          · exact h
+          · exact trans _ _ _ h (rel_of_pairwise_cons h₂ m)
+        · exact ih₁ _ h₁.tail h₂
+      · apply Pairwise.cons
+        · intro z m
+          rw [mem_merge, mem_cons] at m
+          rcases m with (⟨rfl|m⟩|m)
+          · exact total _ _ (by simpa using h)
+          · exact trans _ _ _ (total _ _ (by simpa using h)) (rel_of_pairwise_cons h₁ m)
+          · exact rel_of_pairwise_cons h₂ m
+        · exact ih₂ h₂.tail
+
+theorem splitInTwo_fst_sorted (l : { l : List α // l.length = n }) (h : Sorted le l.1) : Sorted le (splitInTwo l).1.1 := by
+  rw [splitInTwo_fst]
+  exact h.take
+
+theorem splitInTwo_snd_sorted (l : { l : List α // l.length = n }) (h : Sorted le l.1) : Sorted le (splitInTwo l).2.1 := by
+  rw [splitInTwo_snd]
+  exact h.drop
+
+theorem splitInTwo_fst_le_splitInTwo_snd {l : { l : List α // l.length = n }} (h : Sorted le l.1) :
+    ∀ a b, a ∈ (splitInTwo l).1.1 → b ∈ (splitInTwo l).2.1 → le a b := by
+  rw [splitInTwo_fst, splitInTwo_snd]
+  intro a b ma mb
+  exact h.rel_of_mem_take_of_mem_drop ma mb
+
+theorem merge_of_le : ∀ {xs ys : List α} (_ : ∀ a b, a ∈ xs → b ∈ ys → le a b),
+    merge le xs ys = xs ++ ys
+  | [], ys, _
+  | xs, [], _ => by simp [merge]
+  | x :: xs, y :: ys, h => by
+    simp only [merge, cons_append]
+    rw [if_pos, merge_of_le]
+    · intro a b ma mb
+      exact h a b (mem_cons_of_mem _ ma) mb
+    · exact h x y (mem_cons_self _ _) (mem_cons_self _ _)
+
+def stable_le (le : α → α → Bool) (a b : Nat × α) : Bool :=
+  if le a.2 b.2 then if le b.2 a.2 then a.1 ≤ b.1 else true else false
+
+theorem stable_le_trans (trans : ∀ a b c, le a b → le b c → le a c)
+    (a b c : Nat × α) : stable_le le a b → stable_le le b c → stable_le le a c := by
+  simp only [stable_le]
+  split <;> split <;> split <;> rename_i ab₂ ba₂ bc₂
+  · simp_all
+    intro ab₁
+    intro h
+    refine ⟨trans _ _ _ ab₂ bc₂, ?_⟩
+    rcases h with (cd₂ | bc₁)
+    · exact Or.inl (Decidable.byContradiction
+        (fun ca₂ => by simp_all [trans _ _ _ (by simpa using ca₂) ab₂]))
+    · exact Or.inr (Nat.le_trans ab₁ bc₁)
+  · simp_all
+  · simp_all
+    intro h
+    refine ⟨trans _ _ _ ab₂ bc₂, ?_⟩
+    left
+    rcases h with (cb₂ | _)
+    · exact (Decidable.byContradiction
+        (fun ca₂ => by simp_all [trans _ _ _ (by simpa using ca₂) ab₂]))
+    · exact (Decidable.byContradiction
+        (fun ca₂ => by simp_all [trans _ _ _ bc₂ (by simpa using ca₂)]))
+  · simp_all
+  · simp_all
+  · simp_all
+  · simp_all
+  · simp_all
+
+theorem stable_le_total (total : ∀ a b, !le a b → le b a)
+    (a b : Nat × α) : !stable_le le a b → stable_le le b a := by
+  simp only [stable_le]
+  split <;> split
+  · simpa using Nat.le_of_lt
+  · simp
+  · simp
+  · simp_all [total a.2 b.2]
+
+theorem splitInTwo_cons_cons_enumFrom_fst (i : Nat) (l : List α) :
+    (splitInTwo ⟨(i, a) :: (i+1, b) :: l.enumFrom (i+2), rfl⟩).1.1 =
+      (splitInTwo ⟨a :: b :: l, rfl⟩).1.1.enumFrom i := by
+  simp only [length_cons, splitInTwo_fst, enumFrom_length]
+  ext1 j
+  rw [getElem?_take, getElem?_enumFrom, getElem?_take]
+  split
+  · rw [getElem?_cons, getElem?_cons, getElem?_cons, getElem?_cons]
+    split
+    · simp; omega
+    · split
+      · simp; omega
+      · simp only [getElem?_enumFrom]
+        congr
+        ext <;> simp; omega
+  · simp
+
+theorem splitInTwo_cons_cons_enumFrom_snd (i : Nat) (l : List α) :
+    (splitInTwo ⟨(i, a) :: (i+1, b) :: l.enumFrom (i+2), rfl⟩).2.1 =
+      (splitInTwo ⟨a :: b :: l, rfl⟩).2.1.enumFrom (i+(l.length+3)/2) := by
+  simp only [length_cons, splitInTwo_snd, enumFrom_length]
+  ext1 j
+  rw [getElem?_drop, getElem?_enumFrom, getElem?_drop]
+  rw [getElem?_cons, getElem?_cons, getElem?_cons, getElem?_cons]
+  split
+  · simp; omega
+  · split
+    · simp; omega
+    · simp only [getElem?_enumFrom]
+      congr
+      ext <;> simp; omega
+
+theorem merge_stable : ∀ (xs ys) (_ : ∀ x y, x ∈ xs → y ∈ ys → x.1 ≤ y.1),
+    (merge (stable_le le) xs ys).map (·.2) = merge le (xs.map (·.2)) (ys.map (·.2))
+  | [], ys, _ => by simp [merge]
+  | xs, [], _ => by simp [merge]
+  | (i, x) :: xs, (j, y) :: ys, h => by
+    simp only [merge, stable_le, map_cons]
+    split <;> rename_i w
+    · rw [if_pos (by simp [h _ _ (mem_cons_self ..) (mem_cons_self ..)])]
+      simp only [map_cons, cons.injEq, true_and]
+      rw [merge_stable, map_cons]
+      exact fun x' y' mx my => h x' y' (mem_cons_of_mem (i, x) mx) my
+    · simp only [↓reduceIte, map_cons, cons.injEq, true_and]
+      rw [merge_stable, map_cons]
+      exact fun x' y' mx my => h x' y' mx (mem_cons_of_mem (j, y) my)
+
+theorem merge_perm_append : ∀ {xs ys : List α}, merge le xs ys ~ xs ++ ys
+  | [], ys => by simp [merge]
+  | xs, [] => by simp [merge]
+  | x :: xs, y :: ys => by
+    simp only [merge]
+    split
+    · exact merge_perm_append.cons x
+    · exact (merge_perm_append.cons y).trans
+        ((Perm.swap x y _).trans (perm_middle.symm.cons x))
+
+variable (le) in
+theorem mergeSort_perm : ∀ (l : List α), mergeSort le l ~ l
+  | [] => by simp [mergeSort]
+  | [a] => by simp [mergeSort]
+  | a :: b :: xs => by
+    simp only [mergeSort]
+    have : (splitInTwo ⟨a :: b :: xs, rfl⟩).1.1.length < xs.length + 1 + 1 := by simp [splitInTwo_fst]; omega
+    have : (splitInTwo ⟨a :: b :: xs, rfl⟩).2.1.length < xs.length + 1 + 1 := by simp [splitInTwo_snd]; omega
+    exact merge_perm_append.trans
+      (((mergeSort_perm _).append (mergeSort_perm _)).trans
+        (Perm.of_eq (splitInTwo_fst_append_splitInTwo_snd _)))
+termination_by l => l.length
+
+@[simp] theorem mem_mergeSort {a : α} {l : List α} : a ∈ mergeSort le l ↔ a ∈ l :=
+  (mergeSort_perm le l).mem_iff
+
+/--
+The result of `mergeSort` is sorted,
+as long as the comparison function is transitive (`le a b → le b c → le a c`)
+and total in the sense that `le a b ∨ le b a`.
+
+The comparison function need not be irreflexive, i.e. `le a b` and `le b a` is allowed even when `a ≠ b`.
+-/
+theorem mergeSort_sorted
+    (trans : ∀ (a b c : α), le a b → le b c → le a c)
+    (total : ∀ (a b : α), !le a b → le b a) :
+    (l : List α) → (mergeSort le l).Sorted le
+  | [] => by simp [mergeSort]
+  | [a] => by simp [mergeSort]
+  | a :: b :: xs => by
+    have : (splitInTwo ⟨a :: b :: xs, rfl⟩).1.1.length < xs.length + 1 + 1 := by simp [splitInTwo_fst]; omega
+    have : (splitInTwo ⟨a :: b :: xs, rfl⟩).2.1.length < xs.length + 1 + 1 := by simp [splitInTwo_snd]; omega
+    rw [mergeSort]
+    apply merge_sorted @trans @total
+    apply mergeSort_sorted trans total
+    apply mergeSort_sorted trans total
+termination_by l => l.length
+
+/--
+If the input list is already sorted, then `mergeSort` does not change the list.
+-/
+theorem mergeSort_of_sorted : ∀ {l : List α} (_ : Sorted le l), mergeSort le l = l
+  | [], _ => by simp [mergeSort]
+  | [a], _ => by simp [mergeSort]
+  | a :: b :: xs, h => by
+    have : (splitInTwo ⟨a :: b :: xs, rfl⟩).1.1.length < xs.length + 1 + 1 := by simp [splitInTwo_fst]; omega
+    have : (splitInTwo ⟨a :: b :: xs, rfl⟩).2.1.length < xs.length + 1 + 1 := by simp [splitInTwo_snd]; omega
+    rw [mergeSort]
+    rw [mergeSort_of_sorted (splitInTwo_fst_sorted ⟨a :: b :: xs, rfl⟩ h)]
+    rw [mergeSort_of_sorted (splitInTwo_snd_sorted ⟨a :: b :: xs, rfl⟩ h)]
+    rw [merge_of_le (splitInTwo_fst_le_splitInTwo_snd h)]
+    rw [splitInTwo_fst_append_splitInTwo_snd]
+termination_by l => l.length
+
+/--
+This merge sort algorithm is stable,
+in the sense that breaking ties in the ordering function using the position in the list
+has no effect on the output.
+
+That is, elements which are equal with respect to the ordering function will remain
+in the same order in the output list as they were in the input list.
+
+See also:
+* `mergeSort_stable`: if `c <+ l` and `c.Pairwise le`, then `c <+ mergeSort le l`.
+* `mergeSort_stable_pair`: if `[a, b] <+ l` and `le a b`, then `[a, b] <+ mergeSort le l`)
+-/
+theorem mergeSort_enum {l : List α} :
+    (mergeSort (stable_le le) (l.enum)).map (·.2) = mergeSort le l :=
+  go 0 l
+where go : ∀ (i : Nat) (l : List α),
+    (mergeSort (stable_le le) (l.enumFrom i)).map (·.2) = mergeSort le l
+  | _, []
+  | _, [a] => by simp [mergeSort]
+  | _, a :: b :: xs => by
+    have : (splitInTwo ⟨a :: b :: xs, rfl⟩).1.1.length < xs.length + 1 + 1 := by simp [splitInTwo_fst]; omega
+    have : (splitInTwo ⟨a :: b :: xs, rfl⟩).2.1.length < xs.length + 1 + 1 := by simp [splitInTwo_snd]; omega
+    simp only [mergeSort, enumFrom]
+    rw [splitInTwo_cons_cons_enumFrom_fst]
+    rw [splitInTwo_cons_cons_enumFrom_snd]
+    rw [merge_stable]
+    · rw [go, go]
+    · simp only [mem_mergeSort, Prod.forall]
+      intros j x k y mx my
+      have := mem_enumFrom mx
+      have := mem_enumFrom my
+      simp_all
+      omega
+termination_by _ l => l.length
+
+theorem eq_middle_of_mem {l : List α} : a ∈ l → ∃ l₁ l₂, l = l₁ ++ a :: l₂
+  | .head l => ⟨[], l, by simp⟩
+  | .tail a h => by
+    obtain ⟨l₁, l₂, rfl⟩ := eq_middle_of_mem h
+    exact ⟨a :: l₁, l₂, by simp⟩
+
+theorem Perm.eq_of_sorted : ∀ {l₁ l₂ : List α}
+    (_ : ∀ a b, a ∈ l₁ → b ∈ l₂ → le a b → le b a → a = b)
+    (_ : l₁.Sorted le) (_ : l₂.Sorted le) (_ : l₁ ~ l₂), l₁ = l₂
+  | [], [], _, _, _, _ => rfl
+  | [], b :: l₂, _, _, _, h => by simp_all
+  | a :: l₁, [], _, _, _, h => by simp_all
+  | a :: l₁, b :: l₂, w, h₁, h₂, h => by
+    have am : a ∈ b :: l₂ := h.subset (mem_cons_self _ _)
+    have bm : b ∈ a :: l₁ := h.symm.subset (mem_cons_self _ _)
+    have ab : a = b := by
+      simp only [mem_cons] at am
+      rcases am with rfl | am
+      · rfl
+      · simp only [mem_cons] at bm
+        rcases bm with rfl | bm
+        · rfl
+        · exact w _ _ (mem_cons_self _ _) (mem_cons_self _ _)
+            (rel_of_pairwise_cons h₁ bm) (rel_of_pairwise_cons h₂ am)
+    subst ab
+    simp only [perm_cons] at h
+    have := Perm.eq_of_sorted ?_ h₁.tail h₂.tail h
+    simp_all
+    intro a b ha hb
+    exact w a b (mem_cons_of_mem _ ha) (mem_cons_of_mem _ hb)
+
+theorem mergeSort_cons {le : α → α → Bool}
+    (trans : ∀ (a b c : α), le a b → le b c → le a c)
+    (total : ∀ (a b : α), !le a b → le b a)
+    (a : α) (l : List α) :
+    ∃ l₁ l₂, mergeSort le (a :: l) = l₁ ++ a :: l₂ ∧ mergeSort le l = l₁ ++ l₂ ∧
+      ∀ b, b ∈ l₁ → !le a b := by
+  rw [← mergeSort_enum]
+  rw [enum_cons]
+  have nd : Nodup ((a :: l).enum.map (·.1)) := by rw [enum_map_fst]; exact nodup_range _
+  have m₁ : (0, a) ∈ mergeSort (stable_le le) ((a :: l).enum) :=
+    mem_mergeSort.mpr (mem_cons_self _ _)
+  obtain ⟨l₁, l₂, h⟩ := eq_middle_of_mem m₁
+  have s := mergeSort_sorted (stable_le_trans trans) (stable_le_total total) ((a :: l).enum)
+  rw [h] at s
+  have p := mergeSort_perm (stable_le le) ((a :: l).enum)
+  rw [h] at p
+  refine ⟨l₁.map (·.2), l₂.map (·.2), ?_, ?_, ?_⟩
+  · simpa using congrArg (·.map (·.2)) h
+  · rw [← mergeSort_enum.go 1, ← map_append]
+    congr 1
+    have q : mergeSort (stable_le le) (enumFrom 1 l) ~ l₁ ++ l₂ :=
+      (mergeSort_perm (stable_le le) (enumFrom 1 l)).trans
+        (p.symm.trans perm_middle).cons_inv
+    apply Perm.eq_of_sorted (le := stable_le le)
+    · rintro ⟨i, a⟩ ⟨j, b⟩  ha hb
+      simp only [mem_mergeSort] at ha
+      simp only [← q.mem_iff, mem_mergeSort] at hb
+      simp only [stable_le]
+      simp only [Bool.if_false_right, Bool.and_eq_true, Prod.mk.injEq, and_imp]
+      intro ab h ba h'
+      simp only [Bool.decide_eq_true] at ba
+      replace h : i ≤ j := by simpa [ab, ba] using h
+      replace h' : j ≤ i := by simpa [ab, ba] using h'
+      cases Nat.le_antisymm h h'
+      constructor
+      · rfl
+      · have := mem_enumFrom ha
+        have := mem_enumFrom hb
+        simp_all
+    · exact mergeSort_sorted (stable_le_trans trans) (stable_le_total total) ..
+    · exact s.sublist ((sublist_cons_self (0, a) l₂).append_left l₁)
+    · exact q
+  · intro b m
+    simp only [mem_map, Prod.exists, exists_eq_right] at m
+    obtain ⟨j, m⟩ := m
+    replace p := p.map (·.1)
+    have nd' := nd.perm p.symm
+    rw [map_append] at nd'
+    have j0 := nd'.rel_of_mem_append
+      (mem_map_of_mem (·.1) m) (mem_map_of_mem _ (mem_cons_self _ _))
+    simp only [ne_eq] at j0
+    have r := s.rel_of_mem_append m (mem_cons_self _ _)
+    simp_all [stable_le]
+
+/--
+Another statement of stability of merge sort.
+If `c` is a sorted sublist of `l`,
+then `c` is still a sublist of `mergeSort le l`.
+-/
+theorem mergeSort_stable
+    (trans : ∀ (a b c : α), le a b → le b c → le a c)
+    (total : ∀ (a b : α), !le a b → le b a) :
+    ∀ {c : List α} (_ : c.Sorted le) (_ : c <+ l),
+    c <+ mergeSort le l
+  | _, _, .slnil => nil_sublist _
+  | c, hc, @Sublist.cons _ _ l a h => by
+    obtain ⟨l₁, l₂, h₁, h₂, -⟩ := mergeSort_cons trans total a l
+    rw [h₁]
+    have h' := mergeSort_stable trans total hc h
+    rw [h₂] at h'
+    exact h'.middle a
+  | _, _, @Sublist.cons₂ _ l₁ l₂ a h => by
+    rename_i hc
+    obtain ⟨l₃, l₄, h₁, h₂, h₃⟩ := mergeSort_cons trans total a l₂
+    rw [h₁]
+    have h' := mergeSort_stable trans total hc.tail h
+    rw [h₂] at h'
+    simp only [Bool.not_eq_true', tail_cons] at h₃ h'
+    exact
+      sublist_append_of_sublist_right (Sublist.cons₂ a
+        ((fun w => Sublist.of_sublist_append_right w h') fun b m₁ m₃ =>
+          (Bool.eq_not_self true).mp ((rel_of_pairwise_cons hc m₁).symm.trans (h₃ b m₃))))
+
+
+/--
+Another statement of stability of merge sort.
+If a pair `[a, b]` is a sublist of `l` and `le a b`,
+then `[a, b]` is still a sublist of `mergeSort le l`.
+-/
+theorem mergeSort_stable_pair
+    (trans : ∀ (a b c : α), le a b → le b c → le a c)
+    (total : ∀ (a b : α), !le a b → le b a)
+    (hab : le a b) (h : [a, b] <+ l) : [a, b] <+ mergeSort le l :=
+  mergeSort_stable trans total (pairwise_pair.mpr hab) h
+
+end List
+
+open List
