src/Init/Data/List/Sort/Lemmas.lean
@@ -5,5 +5,3 @@ Authors: Kim Morrison
 -/
 prelude
 import Init.Data.List.Sort.Basic
-import Init.Data.List.Sort.Impl
-import Init.Data.List.Sort.Lemmas
