tests/lean/run/mergeSort.lean
@@ -1,0 +1,25 @@
+open List
+
+unseal mergeSort merge in
+example : mergeSort (· ≤ ·) [3, 1, 4, 1, 5, 9, 2, 6, 5, 3, 5] = [1, 1, 2, 3, 3, 4, 5, 5, 5, 6, 9] :=
+  rfl
+
+unseal mergeSort merge in
+example : mergeSort (fun x y => x/10 ≤ y/10) [3, 100 + 1, 4, 100 + 1, 5, 100 + 9, 2, 10 + 6, 5, 10 + 3, 5] = [3, 4, 5, 2, 5, 5, 16, 13, 101, 101, 109] :=
+  rfl
+
+unseal mergeSortTR.run mergeTR.go in
+example : mergeSortTR (· ≤ ·) [3, 1, 4, 1, 5, 9, 2, 6, 5, 3, 5] = [1, 1, 2, 3, 3, 4, 5, 5, 5, 6, 9] :=
+  rfl
+
+unseal mergeSortTR.run mergeTR.go in
+example : mergeSortTR (fun x y => x/10 ≤ y/10) [3, 100 + 1, 4, 100 + 1, 5, 100 + 9, 2, 10 + 6, 5, 10 + 3, 5] = [3, 4, 5, 2, 5, 5, 16, 13, 101, 101, 109] :=
+  rfl
+
+unseal mergeSortTR₂.run mergeTR.go in
+example : mergeSortTR₂ (· ≤ ·) [3, 1, 4, 1, 5, 9, 2, 6, 5, 3, 5] = [1, 1, 2, 3, 3, 4, 5, 5, 5, 6, 9] :=
+  rfl
+
+unseal mergeSortTR₂.run mergeTR.go in
+example : mergeSortTR₂ (fun x y => x/10 ≤ y/10) [3, 100 + 1, 4, 100 + 1, 5, 100 + 9, 2, 10 + 6, 5, 10 + 3, 5] = [3, 4, 5, 2, 5, 5, 16, 13, 101, 101, 109] :=
+  rfl
